feat: Implement structural recursion for inductive predicates.

tests/lean/run/structuralRec1.lean
@@ -1,6 +1,16 @@
+inductive PList (α : Type) : Prop
+| nil
+| cons : α → PList α → PList α
+
+infixr:67 " ::: " => PList.cons
+
 def map {α β} (f : α → β) : List α → List β
 | []    => []
 | a::as => f a :: map f as
+
+def pmap {α β} (f : α → β) : PList α → PList β
+| PList.nil => PList.nil
+| a:::as => f a ::: pmap f as
 
 theorem ex1 : map Nat.succ [1] = [2] :=
 rfl
@@ -23,6 +33,13 @@ let rec loop : List α → List β
  | a::as => f a :: loop as;
 loop as
 
+def pmap2 {α β} (f : α → β) (as : PList α) : PList β :=
+let rec loop : PList α → PList β
+ | PList.nil    => PList.nil 
+ | a:::as => f a ::: loop as;
+loop as
+
+
 theorem ex6 {α β} (f : α → β) (a : α) (as : List α) : map2 f (a::as) = (f a) :: map2 f as :=
 rfl
 
@@ -34,6 +51,15 @@ match xs with
   match xs with
   | []    => []
   | x::xs => (y + x) :: foo xs
+
+def pfoo (xs : PList Nat) : PList Nat :=
+match xs with
+| PList.nil   => PList.nil
+| x:::xs =>
+  let y := 2 * x;
+  match xs with
+  | PList.nil    => PList.nil 
+  | x:::xs => (y + x) ::: pfoo xs
 
 #eval foo [1, 2, 3, 4]
 
@@ -50,8 +76,22 @@ else
   | []    => []
   | y::ys => (y + x/2 + 1) :: bla (x/2) ys
 
+def pbla (x : Nat) (ys : PList Nat) : PList Nat :=
+if x % 2 == 0 then
+  match ys with
+  | PList.nil    => PList.nil 
+  | y:::ys => (y + x/2) ::: pbla (x/2) ys
+else
+  match ys with
+  | PList.nil    => PList.nil 
+  | y:::ys => (y + x/2 + 1) ::: pbla (x/2) ys
+
 theorem blaEq (y : Nat) (ys : List Nat) : bla 4 (y::ys) = (y+2) :: bla 2 ys :=
 rfl
+
+inductive PNat : Prop
+| zero
+| succ : PNat → PNat
 
 def f : Nat → Nat → Nat
  | 0, y   => y
@@ -59,6 +99,13 @@ def f : Nat → Nat → Nat
    match f x y with
    | 0 => f x y
    | v => f x v + 1
+
+def pf : PNat → PNat → PNat
+ | PNat.zero, y   => y
+ | PNat.succ x, y =>
+   match pf x y with
+   | PNat.zero => pf x y
+   | v => PNat.succ $ pf x v
 
 def g (xs : List Nat) : Nat :=
   match xs with
@@ -68,6 +115,14 @@ def g (xs : List Nat) : Nat :=
     | [] => 1
     | _ => g ys + 1
 
+def pg (xs : PList Nat) : True :=
+  match xs with
+  | PList.nil => True.intro
+  | y:::ys =>
+    match ys with
+    | PList.nil => True.intro
+    | _ => pg ys 
+
 def aux : Nat → Nat → Nat
  | 0, y   => y
  | x+1, y =>
@@ -75,7 +130,72 @@ def aux : Nat → Nat → Nat
    | 0 => f x y
    | v => f x v + 1
 
+def paux : PNat → PNat → PNat
+ | PNat.zero, y   => y
+ | PNat.succ x, y =>
+   match pf x y with
+   | PNat.zero => pf x y
+   | v => pf x v + 1
+
 theorem ex (x y : Nat) : f x y = aux x y := by
   cases x
   rfl
   rfl
+
+axiom F : Nat → Nat
+
+inductive is_nat : Nat -> Prop
+| Z : is_nat 0
+| S {n} : is_nat n → is_nat (F n)
+
+axiom P : Nat → Prop
+axiom F0 : P 0
+axiom F1 : P (F 0)
+axiom FS {n : Nat} : P n → P (F (F n))
+
+-- set_option trace.Elab.definition.structural true in
+theorem «nested recursion» : ∀ {n}, is_nat n → P n
+| _, is_nat.Z => F0
+| _, is_nat.S is_nat.Z => F1
+| _, is_nat.S (is_nat.S h) => FS («nested recursion» h)
+
+theorem «reordered discriminants» : ∀ n, is_nat n → Nat → P n := fun n hn m => 
+match n, m, hn with
+| _, _, is_nat.Z => F0
+| _, _, is_nat.S is_nat.Z => F1
+| _, m, is_nat.S (is_nat.S h) => FS («reordered discriminants» _ h m)
+
+def «unsupported nesting» (xs : List Nat) : True :=
+  match xs with
+  | List.nil => True.intro
+  | y::ys =>
+    match ys with
+    | List.nil      => True.intro
+    | _::_::zs      => «unsupported nesting» zs 
+    | zs            => «unsupported nesting» ys 
+
+def «unsupported nesting, predicate» (xs : PList Nat) : True :=
+  match xs with
+  | PList.nil => True.intro
+  | y:::ys =>
+    match ys with
+    | PList.nil      => True.intro
+    | _:::_:::zs     => «unsupported nesting, predicate» zs 
+    | zs             => «unsupported nesting, predicate» ys 
+
+
+def f1 (xs : List Nat) : Nat :=
+match xs with
+| [] => 0
+| x::xs =>
+  match xs with
+  | []  => 0
+  | _ => f1 xs + 1
+
+def pf1 (xs : PList Nat) : True :=
+match xs with
+| PList.nil => True.intro
+| x:::xs =>
+  match xs with
+  | PList.nil  => True.intro
+  | _ => pf1 xs 
